Okay, we've gotten a construct for time and an unhalting Turing machine that presumably eventually (or somehow) cycles back to its origin starting state. We got this from hacking the definition of equivalence. We will take a step back now and derive it a little more formally. It is stupid, but perhaps there's nothing stopping us from doing this re-defining and obtaining a deductive logic from which cosmogenesis could theoretically make sense, noting: the Big Bang Theory is not a cosmogenesis theory and chronicles the early moments and evolution of the observable beginning of the universe. An un-mythological cosmogenesis theory has, perhaps, yet to be proposed in the scope of deduction. Myths, such as my favorite being Tolkien's cosmogenesis allegory (yes it is an allegory) of the universe arising from a musical theme, do exist and perhaps have extreme truth to them, all.

**Definition 1.** Axiom $A$ "is true" or $A$ "exists": $\exists A$.

**Axiom 1.** A definition $A = B$ is true. 

**Definition 2.** Equivalence $A = B$ means $A \rightarrow_n B$ and $B \rightarrow_m A$ in $n, m \in \mathbb{N}$ deductive steps.

**Definition 3.** Implication $A \rightarrow_1 B$ means that if $A$ is true ($\exists A$), $B$ is true ($\exists B$) upon the immediate next deductive step.

**Definition 4.** Deduction/proof $A \rightarrow_n B$ means that if $A$ is true ($\exists A$), $B$ is true ($\exists B$) upon $n$ deductive steps.

We have now defined proof.

This definition, while hacky, generalizes to every other definition and deductive process.

It is more general.

---

$A$ and $B$ are any statement whose contents and operators are defined.

This can maybe be written:

**Definition 1.** $($ Axiom  $A ) = (\exists A)$.

**Definition 2.** $($ Definition $A = B) = (\exists (A = B)$. 

**Definition 3.** $($ Equivalence $A = B) = (A \rightarrow_n B, B \rightarrow_m A, n, m \in \mathbb{N})$, where $n, m$ are deductive steps, meaning $n, m$ statements must be deduced between $A$ and $B$ and $B$ and $A$ respectively.

**Definition 4.** $($ Implication $A \rightarrow_1 B) = (\exists A \rightarrow_1 \exists B)$.

**Definition 5.** $($ Deduction/proof $A \rightarrow_n B) = (\exists A \rightarrow_n \exists B)$.
